src/AwsCryptographicMaterialProviders/Commitment.dfy
@@ -16,31 +16,26 @@ module {:extern "Dafny.Aws.Crypto.MaterialProviders.Commitment"} MaterialProvide
    * Validates that the given algorithm is allowed by the the given commitment policy
    * during encryption
    */
-  method ValidateCommitmentPolicyOnEncrypt(
-    algorithm: Option<Crypto.AlgorithmSuiteId>,
+  function method ValidateCommitmentPolicyOnEncrypt(
+    algorithm: Crypto.AlgorithmSuiteId,
     commitmentPolicy: Crypto.CommitmentPolicy
-  )
+  ):
     // Bool return type on success is somewhat arbitrary; mainly we care about
     // success/failure
-    returns (res: Result<bool, string>)
+    (res: Result<bool, string>)
 
-    // If an algorithm suite was not provided it cannot conflict with the
-    // commitment policy
-    ensures algorithm.None? ==> res.Success?
-
-    // Commitment policy forbids encrypting with commitment but the
+    // Failure: Commitment policy forbids encrypting with commitment but the
     // algorithm provides it
     ensures
       (
         && commitmentPolicy == Crypto.FORBID_ENCRYPT_ALLOW_DECRYPT
-        && algorithm.Some?
-        && var suite := AlgorithmSuites.GetSuite(algorithm.value);
+        && var suite := AlgorithmSuites.GetSuite(algorithm);
         && !suite.commitment.None?
       )
     ==>
       res.Failure?
 
-    // Commitment policy requires encrypting with commitment but the
+    // Failure: Commitment policy requires encrypting with commitment but the
     // algorithm does not provide it
     ensures
       (
@@ -48,80 +43,112 @@ module {:extern "Dafny.Aws.Crypto.MaterialProviders.Commitment"} MaterialProvide
           || commitmentPolicy == Crypto.REQUIRE_ENCRYPT_ALLOW_DECRYPT
           || commitmentPolicy == Crypto.REQUIRE_ENCRYPT_REQUIRE_DECRYPT
         )
-        && algorithm.Some?
-        && var suite := AlgorithmSuites.GetSuite(algorithm.value);
+        && var suite := AlgorithmSuites.GetSuite(algorithm);
         && suite.commitment.None?
       )
     ==>
       res.Failure?
+
+    // Success: Commitment policy requires encrypting with commitment and the
+    // algorithm provides it
+    ensures
+      (
+        && (
+          || commitmentPolicy == Crypto.REQUIRE_ENCRYPT_ALLOW_DECRYPT
+          || commitmentPolicy == Crypto.REQUIRE_ENCRYPT_REQUIRE_DECRYPT
+        )
+        && var suite := AlgorithmSuites.GetSuite(algorithm);
+        && !suite.commitment.None?
+      )
+    ==>
+      res.Success?
+
+    // Success: Commitment policy forbids encrypting with commitment and the
+    // algorithm does not provide it
+    ensures
+      (
+        && commitmentPolicy == Crypto.FORBID_ENCRYPT_ALLOW_DECRYPT
+        && var suite := AlgorithmSuites.GetSuite(algorithm);
+        && suite.commitment.None?
+      )
+    ==>
+      res.Success?
   {
-    if algorithm.None? {
-      return Success(true);
-    }
-
-    var suite := AlgorithmSuites.GetSuite(algorithm.value);
-
+    var suite := AlgorithmSuites.GetSuite(algorithm);
     if
       && commitmentPolicy == Crypto.FORBID_ENCRYPT_ALLOW_DECRYPT
       && !suite.commitment.None?
-    {
-      return Failure("Configuration conflict. Commitment policy requires only non-committing algorithm suites");
-    }
-
-    if
+    then
+      Failure("Configuration conflict. Commitment policy requires only non-committing algorithm suites")
+    else if
       && (
           || commitmentPolicy == Crypto.REQUIRE_ENCRYPT_ALLOW_DECRYPT
           || commitmentPolicy == Crypto.REQUIRE_ENCRYPT_REQUIRE_DECRYPT
          )
       && suite.commitment.None?
-    {
-      return Failure("Configuration conflict. Commitment policy requires only committing algorithm suites");
-    }
-
-    return Success(true);
+    then
+      Failure("Configuration conflict. Commitment policy requires only committing algorithm suites")
+    else
+      Success(true)
   }
 
   /*
    * Validates that the given algorithm is allowed by the the given commitment policy
    * during decryption
    */
-  method ValidateCommitmentPolicyOnDecrypt(
-    algorithm: Option<Crypto.AlgorithmSuiteId>,
+  function method ValidateCommitmentPolicyOnDecrypt(
+    algorithm: Crypto.AlgorithmSuiteId,
     commitmentPolicy: Crypto.CommitmentPolicy
-  )
+  ):
     // Bool return type on success is somewhat arbitrary; mainly we care about
     // success/failure
-    returns (res: Result<bool, string>)
+    (res: Result<bool, string>)
 
-    // If an algorithm suite was not provided it cannot conflict with the
-    // commitment policy
-    ensures algorithm.None? ==> res.Success?
-
-    // Commitment policy requires decrypting with commitment but the
+    // Failure: Commitment policy requires decrypting with commitment but the
     // algorithm does not provide it
     ensures
       (
         && commitmentPolicy == Crypto.REQUIRE_ENCRYPT_REQUIRE_DECRYPT
-        && algorithm.Some?
-        && var suite := AlgorithmSuites.GetSuite(algorithm.value);
+        && var suite := AlgorithmSuites.GetSuite(algorithm);
         && suite.commitment.None?
       )
     ==>
       res.Failure?
-  {
-    if algorithm.None? {
-      return Success(true);
-    }
 
-    var suite := AlgorithmSuites.GetSuite(algorithm.value);
+    // Success: Commitment policy requires decrypting with commitment and
+    // our algorithm provides it
+    ensures
+      (
+        && commitmentPolicy == Crypto.REQUIRE_ENCRYPT_REQUIRE_DECRYPT
+        && var suite := AlgorithmSuites.GetSuite(algorithm);
+        && !suite.commitment.None?
+      )
+    ==>
+      res.Success?
+
+    // Success: Commitment policy does not require decrypting with commitment and
+    // our algorithm does not provide it
+    ensures
+      (
+        && (
+            || commitmentPolicy == Crypto.FORBID_ENCRYPT_ALLOW_DECRYPT
+            || commitmentPolicy == Crypto.REQUIRE_ENCRYPT_ALLOW_DECRYPT
+           )
+        && var suite := AlgorithmSuites.GetSuite(algorithm);
+        && suite.commitment.None?
+      )
+    ==>
+      res.Success?
+
+  {
+    var suite := AlgorithmSuites.GetSuite(algorithm);
 
     if
       && commitmentPolicy == Crypto.REQUIRE_ENCRYPT_REQUIRE_DECRYPT
       && suite.commitment.None?
-    {
-      return Failure("Configuration conflict. Commitment policy requires only committing algorithm suites");
-    }
-
-    return Success(true);
+    then
+      Failure("Configuration conflict. Commitment policy requires only committing algorithm suites")
+    else
+      Success(true)
   }
 }
