src/AwsCryptographicMaterialProviders/Defaults.dfy
@@ -7,8 +7,8 @@ module {:extern "Defaults"} Defaults {
 
   /* Returns the default algorithm suite for the given commitment policy */
   // TODO: move to default commitment algorithms once supported by the rest of the code
-  method GetAlgorithmSuiteForCommitmentPolicy(commitmentPolicy: Crypto.CommitmentPolicy)
-    returns (res: Crypto.AlgorithmSuiteId)
+  function method GetAlgorithmSuiteForCommitmentPolicy(commitmentPolicy: Crypto.CommitmentPolicy):
+    (res: Crypto.AlgorithmSuiteId)
     ensures
       commitmentPolicy == Crypto.FORBID_ENCRYPT_ALLOW_DECRYPT
       ==>
@@ -20,12 +20,8 @@ module {:extern "Defaults"} Defaults {
       //res == Crypto.ALG_AES_256_GCM_HKDF_SHA512_COMMIT_KEY_ECDSA_P384
       res == Crypto.ALG_AES_256_GCM_IV12_TAG16_HKDF_SHA384_ECDSA_P384
   {
-    if commitmentPolicy == Crypto.FORBID_ENCRYPT_ALLOW_DECRYPT {
-      return Crypto.ALG_AES_256_GCM_IV12_TAG16_HKDF_SHA384_ECDSA_P384;
-    } else if commitmentPolicy == Crypto.REQUIRE_ENCRYPT_ALLOW_DECRYPT ||
-              commitmentPolicy == Crypto.REQUIRE_ENCRYPT_REQUIRE_DECRYPT {
-      return Crypto.ALG_AES_256_GCM_IV12_TAG16_HKDF_SHA384_ECDSA_P384;
-      //return Crypto.ALG_AES_256_GCM_HKDF_SHA512_COMMIT_KEY_ECDSA_P384;
-    }
+    if commitmentPolicy == Crypto.FORBID_ENCRYPT_ALLOW_DECRYPT then
+      Crypto.ALG_AES_256_GCM_IV12_TAG16_HKDF_SHA384_ECDSA_P384 else
+      Crypto.ALG_AES_256_GCM_IV12_TAG16_HKDF_SHA384_ECDSA_P384 // TODO: committing algorithm by default
   }
 }
